PDDL_to_STRIPS.thy
@@ -1,9 +1,11 @@
+ 
 theory PDDL_to_STRIPS
   imports "Classical_Planning.Classical_Abstract_Syntax"
     "Classical_Planning.Classical_Happening_Semantics"
     Tree_Decomp_Grounding_Base.PDDL_Sema_Supplement
     Tree_Decomp_Grounding_Base.STRIPS_Sema_Supplement
     Tree_Decomp_Grounding_Base.Normalization_Definitions
+    Tree_Decomp_Grounding_Base.Numeric_Free
     (* list linorder: *) "HOL-Library.List_Lexorder" "HOL-Library.Char_ord" (* only used to minimize negative literals *)
 begin
 
@@ -23,11 +25,24 @@ text \<open>There are two big differences between normalized ground PDDL and
   seemed easier.
 \<close>
 
-definition "v\<^sub>T \<equiv> ''+'' :: name"
-definition "v\<^sub>F \<equiv> ''-'' :: name"
-abbreviation "vpos p \<equiv> CHR ''+'' # predicate.name p"
-abbreviation "vneg p \<equiv> CHR ''-'' # predicate.name p"
+definition "v\<^sub>T \<equiv> STR ''+'' :: name"
+definition "v\<^sub>F \<equiv> STR ''-'' :: name"
+abbreviation "vpos p \<equiv> STR ''+'' + predicate.name p"
+abbreviation "vneg p \<equiv> STR ''-'' + predicate.name p"
 lemmas vb_defs = v\<^sub>T_def v\<^sub>F_def
+
+lemma lit_prepend_inj: "(s + a = s + b) = (a = b)" for s a b :: name
+  by (metis String.implode_explode_eq plus_literal.rep_eq same_append_eq)
+
+lemma vneg_neq_vpos: "vneg p \<noteq> vpos q"
+proof
+  assume "vneg p = vpos q"
+  hence "literal.explode (STR ''-'' + predicate.name p)
+       = literal.explode (STR ''+'' + predicate.name q)" by simp
+  moreover have "literal.explode (STR ''-'' :: name) = ''-''"
+                "literal.explode (STR ''+'' :: name) = ''+''" by eval+
+  ultimately show False by (simp add: plus_literal.rep_eq)
+qed
 
 text \<open>iceboxed because e.g. "pred_vpos = vpos \<circ> pred" \<close>
 (*fun pred_vpos :: "predicate_decl \<Rightarrow> name" where
@@ -63,17 +78,17 @@ fun atm_as_vneg :: "'a atom formula \<Rightarrow> name" where
 (* add effects take precedence *)
 (* removes duplicates *)
 fun fix_effect :: "'a ast_effect \<Rightarrow> 'a ast_effect" where
-  "fix_effect (Effect add del) = Effect add (filter (\<lambda>x. x \<notin> set add) del)"
+  "fix_effect (Effect add del nums) = Effect add (filter (\<lambda>x. x \<notin> set add) del) nums"
 
-fun as_strips_op :: "ast_action_schema \<Rightarrow> name strips_operator" where
-  "as_strips_op (Action_Schema n args pre eff) =
+fun as_strips_op :: "ast_classical_action_schema \<Rightarrow> name strips_operator" where
+  "as_strips_op (SimpleActionSchema (ActionHead n args) (SimpleActionBody pre eff)) =
   (let eff' = fix_effect eff; add = adds eff'; del = dels eff' in
   \<lparr>
     precondition_of = fmla_as_vars pre
     , add_effects_of = map atm_as_vpos add @ map atm_as_vneg del
     , delete_effects_of = map atm_as_vpos del @ map atm_as_vneg add \<rparr>)"
 
-context ast_problem begin
+context ast_classical_problem begin
 
 abbreviation "strips_ops \<equiv> map as_strips_op (actions D)"
 
@@ -108,26 +123,26 @@ definition as_strips :: "name strips_problem" where
     , initial_of = strips_init
     , goal_of = strips_goal \<rparr>"
 
-definition "restore_pddl_pa op \<equiv>
-  PAction (ac_name (actions D ! the (find_index op strips_ops))) []"
+definition "restore_pddl_pa opp \<equiv>
+  SimplePlanAction (ac_name (actions D ! the (find_index opp strips_ops))) []"
 definition "restore_pddl_plan op_is \<equiv> map restore_pddl_pa op_is"
 
-end text \<open>context ast_problem\<close>
+end text \<open>context ast_classical_problem\<close>
 
 lemmas to_strips_code =
-  ast_problem.vars_defs
-  ast_problem.init_defs
-  ast_problem.strips_goal_def
-  ast_problem.as_strips_def
-  ast_problem.restore_pddl_pa_def
-  ast_problem.restore_pddl_plan_def
+  ast_classical_problem.vars_defs
+  ast_classical_problem.init_defs
+  ast_classical_problem.strips_goal_def
+  ast_classical_problem.as_strips_def
+  ast_classical_problem.restore_pddl_pa_def
+  ast_classical_problem.restore_pddl_plan_def
 declare to_strips_code[code]
 
-value "ast_problem.as_strips" (* checking if code exists *)
+value "ast_classical_problem.as_strips" (* checking if code exists *)
 
 subsection \<open> Alternative definitions \<close>
 
-context ast_problem begin
+context ast_classical_problem begin
 
 lemma as_strips_op_sel [simp]:
   fixes ac
@@ -135,9 +150,13 @@ lemma as_strips_op_sel [simp]:
   shows "precondition_of (as_strips_op ac) = fmla_as_vars (ac_pre ac)"
   "add_effects_of (as_strips_op ac) = map atm_as_vpos (adds eff') @ map atm_as_vneg (dels eff')"
   "delete_effects_of (as_strips_op ac) = map atm_as_vpos (dels eff') @ map atm_as_vneg (adds eff')"
-  apply (cases ac) apply simp_all unfolding as_strips_op.simps Let_def apply simp
-  apply (cases ac) apply simp_all unfolding as_strips_op.simps Let_def eff'_def apply simp
-  apply (cases ac) apply simp_all unfolding as_strips_op.simps Let_def eff'_def by simp
+  apply (cases ac)
+  subgoal for head body by (cases head, cases body) (simp add: Let_def)
+  apply (cases ac)
+  subgoal for head body by (cases head, cases body) (simp add: Let_def eff'_def)
+  apply (cases ac)
+  subgoal for head body by (cases head, cases body) (simp add: Let_def eff'_def)
+  done
 
 lemma as_strips_sel [simp]:
   "as_strips \<^sub>\<V> = strips_vars"
@@ -145,11 +164,11 @@ lemma as_strips_sel [simp]:
   "as_strips \<^sub>I = strips_init"
   "as_strips \<^sub>G = strips_goal"
   unfolding as_strips_def by simp_all
-end text \<open>context ast_problem\<close>
+end text \<open>context ast_classical_problem\<close>
 
 subsection \<open> Formula structures \<close>
 
-context ast_domain begin
+context ast_classical_domain begin
 definition "wf_pred n \<equiv> PredDecl n [] \<in> set (predicates D)"
 fun wf_lit where
   "wf_lit \<bottom> = True" |
@@ -161,11 +180,11 @@ abbreviation "wf_lit_atom F \<equiv> wf_lit F \<and> is_predAtom F"
 (* ? *)
 lemma wf_lit_plus: "wf_lit L \<Longrightarrow> is_lit_plus L"
   by (cases L rule: wf_lit.cases) simp_all
-end text \<open>context ast_domain\<close>
+end text \<open>context ast_classical_domain\<close>
 
 
-(* technically, also holds in ast_domain but easier to prove here with sig_Some *)
-context wf_ast_domain begin
+(* technically, also holds in ast_classical_domain but easier to prove here with sig_Some *)
+context wf_ast_classical_domain begin
 lemma wf_predatom_lit:
   "wf_pred_atom (\<lambda>x. None) (n, args) \<longleftrightarrow> args = [] \<and> wf_pred n"
   (is "?L \<longleftrightarrow> ?R")
@@ -182,15 +201,29 @@ proof -
   finally show ?thesis .
 qed
 
+text \<open>A numeric-free (\<^const>\<open>num_free_fmla\<close>) well-formed literal under the empty type environment
+  is a \<^const>\<open>wf_lit\<close>: the numeric-free hypothesis rules out the \<open>numericXxxAtm\<close> atoms (which
+  \<open>wf_lit\<close> would otherwise reject), an \<open>eqAtm\<close> is impossible under \<open>\<lambda>x. None\<close>
+  (\<open>wf_atom (eqAtm a b)\<close> needs both entities typed), and a \<open>predAtm\<close> must have empty arguments and
+  a declared predicate (@{thm wf_predatom_lit}). The numeric-free hypothesis is the
+  propositional-fragment restriction (see \<^theory>\<open>Tree_Decomp_Grounding_Base.Numeric_Free\<close>); it
+  holds for the grounded+normalized input fed to the STRIPS backend.\<close>
 lemma wf_empty_lit:
-  assumes "is_lit_plus L" "wf_fmla (\<lambda>x. None) L"
+  assumes "num_free_fmla L" "is_lit_plus L" "wf_fmla (\<lambda>x. None) L"
   shows "wf_lit L"
-  using assms wf_predatom_lit[unfolded wf_pred_atom.simps]
-  by (cases L rule: wf_lit.cases) force+
+  using assms
+proof (cases L rule: is_lit_plus.cases)
+  case (3 a) \<comment> \<open>\<open>L = Atom a\<close>\<close>
+  then show ?thesis using assms by (cases a) (auto simp: wf_predatom_lit simp del: wf_pred_atom.simps)
+next
+  case (4 a) \<comment> \<open>\<open>L = \<^bold>\<not> (Atom a)\<close>\<close>
+  then show ?thesis using assms by (cases a) (auto simp: wf_predatom_lit simp del: wf_pred_atom.simps)
+qed auto
+
 
 lemma wf_empty_lits:
-  assumes "is_conj F" "wf_fmla (\<lambda>x. None) F"
-  shows "list_all1 wf_lit (un_and F)"
+  assumes "num_free_fmla F" "is_conj F" "wf_fmla (\<lambda>x. None) F"
+  shows "(\<forall>x \<in> set (un_and F). wf_lit x)"
   using assms wf_empty_lit
   by (induction F) auto
 
@@ -198,11 +231,18 @@ lemma wf_empty_atom:
   assumes "wf_fmla_atom (\<lambda>x. None) L"
   shows "wf_lit_atom L"
 proof -
-  from assms have "is_lit_plus L"
+  from assms have lp: "is_lit_plus L"
     by (cases L rule: wf_fmla_atom.cases) simp_all
-  with assms show ?thesis using wf_empty_lit unfolding wf_fmla_atom_alt by blast
+  from assms have nf: "num_free_fmla L"
+    by (cases L rule: wf_fmla_atom.cases) auto
+  from assms have pa: "is_predAtom L"
+    by (cases L rule: wf_fmla_atom.cases) auto
+  from assms have wff: "wf_fmla (\<lambda>x. None) L"
+    unfolding wf_fmla_atom_alt by simp
+  have "wf_lit L" by (rule wf_empty_lit[OF nf lp wff])
+  with pa show "wf_lit_atom L" by simp
 qed
-end text \<open>context wf_ast_domain\<close>
+end text \<open>context wf_ast_classical_domain\<close>
 
 
 context grounded_problem begin
@@ -219,61 +259,78 @@ lemma ac_tyt_empty:
   assumes "ac \<in> set (actions D)" shows "ac_tyt ac = (\<lambda>x. None)"
 proof -
   from assms have "grounded_ac ac" using grounded_dom grounded_dom_def by blast
-  hence "ac_params ac = []" by (cases ac) simp
-  thus "?thesis"
-    apply (intro ext)
-    subgoal for x
-      using constT_empty by (cases x) simp_all
-    done
+  hence acp: "ac_params ac = []" by (cases ac rule: grounded_ac.cases) auto
+  show ?thesis
+  proof (rule ext)
+    fix x show "ac_tyt ac x = None" by (cases x) (simp_all add: ac_tyt_def acp constT_empty)
+  qed
 qed
 
 lemma (in grounded_normalized_problem) wf_pre_lits:
-  assumes "ac \<in> set (actions D)" shows "list_all1 wf_lit (un_and (ac_pre ac))"
+  assumes "ac \<in> set (actions D)" "num_free_ac ac"
+  shows "(\<forall>x \<in> set (un_and (ac_pre ac)). wf_lit x)"
 proof -
-  have "wf_fmla (\<lambda>x. None) (ac_pre ac)"
-    using assms wf_D(7) ac_tyt_empty wf_action_schema_alt by metis
+  have wfa: "wf_classical_action_schema ac" using assms(1) wf_D(3) by blast
+  have "wf_fmla (ac_tyt ac) (ac_pre ac)"
+    using wfa by (cases ac rule: ast_classical_action_schema_cases_unfold) (auto simp: ac_tyt_def Let_def)
+  hence "wf_fmla (\<lambda>x. None) (ac_pre ac)" using ac_tyt_empty[OF assms(1)] by simp
   moreover have "is_conj (ac_pre ac)"
-    using assms normed_prob
+    using assms(1) normed_prob
     unfolding prec_normed_dom_def by simp
+  moreover have "num_free_fmla (ac_pre ac)"
+    using assms(2) unfolding num_free_ac_def by simp
   ultimately show ?thesis using wf_empty_lits by blast
 qed
 
 lemma wf_eff_lits:
   assumes "ac \<in> set (actions D)"
-  shows "list_all1 wf_lit_atom (adds (ac_eff ac))" (is ?A)
-        "list_all1 wf_lit_atom (dels (ac_eff ac))" (is ?B)
-  using assms ac_tyt_empty
-  using wf_D(7) wf_action_schema_alt wf_effect_alt wf_empty_atom
-    by metis+
+  shows "(\<forall>x \<in> set (adds (ac_eff ac)). wf_lit_atom x)" (is ?A)
+        "(\<forall>x \<in> set (dels (ac_eff ac)). wf_lit_atom x)" (is ?B)
+proof -
+  have wfa: "wf_classical_action_schema ac" using assms wf_D(3) by blast
+  have "wf_effect (ac_tyt ac) (ac_eff ac)"
+    using wfa by (cases ac rule: ast_classical_action_schema_cases_unfold) (auto simp: ac_tyt_def Let_def)
+  hence eff: "wf_effect (\<lambda>x. None) (ac_eff ac)" using ac_tyt_empty[OF assms] by simp
+  show ?A using eff wf_empty_atom by (cases "ac_eff ac") auto
+  show ?B using eff wf_empty_atom by (cases "ac_eff ac") auto
+qed
 
 lemma wf_init_lits:
-  shows "list_all1 wf_lit_atom (init P)"
-  using wf_empty_atom wf_P(4)
-  unfolding wf_world_model_def objT_empty by blast
+  assumes "\<forall>f \<in> set (init P). num_free_fmla f"
+  shows "(\<forall>x \<in> set (init P). wf_lit_atom x)"
+proof (rule ballI)
+  fix x assume x: "x \<in> set (init P)"
+  from x wf_P(4) have disj: "wf_fmla_atom objT x \<or> wf_func_assign x" by blast
+  from x assms have nf: "num_free_fmla x" by blast
+  have "wf_fmla_atom objT x"
+    using disj nf by (cases x rule: wf_func_assign.cases) auto
+  thus "wf_lit_atom x" using wf_empty_atom unfolding objT_empty by blast
+qed
 
 end text \<open>context wf_grounded_problem \<close>
 
 lemma (in grounded_normalized_problem) wf_goal_lits:
-  "list_all1 wf_lit (un_and (goal P))"
-  using objT_empty wf_P(5) wf_empty_lits normed_prob by auto
+  assumes "num_free_fmla (goal P)"
+  shows "(\<forall>x \<in> set (un_and (goal P)). wf_lit x)"
+  using assms objT_empty wf_P(5) wf_empty_lits normed_prob by auto
 
 subsection \<open> STRIPS task is WF \<close>
 
-context ast_problem begin
+context ast_classical_problem begin
 
-lemma (in ast_problem) wf_lit_covered:
+lemma (in ast_classical_problem) wf_lit_covered:
   assumes "wf_lit F"
   shows "lit_as_var F \<in> set strips_vars"
   unfolding vars_defs
   using assms wf_pred_def by (cases F rule: wf_lit.cases) force+
 
-lemma (in ast_problem) wf_lit_goal_covered:
+lemma (in ast_classical_problem) wf_lit_goal_covered:
   assumes "wf_lit F"
   shows "fst (lit_as_goal F) \<in> set strips_vars"
   unfolding vars_defs
   using assms wf_pred_def by (cases F rule: wf_lit.cases) force+
 
-lemma (in ast_problem) wf_lit_atom_covered:
+lemma (in ast_classical_problem) wf_lit_atom_covered:
   assumes "wf_lit_atom F" shows
     "atm_as_vpos F \<in> set pos_vars"
     "atm_as_vneg F \<in> set neg_vars"
@@ -282,28 +339,28 @@ lemma (in ast_problem) wf_lit_atom_covered:
   using assms wf_pred_def apply (cases F rule: wf_lit.cases) apply force+
   done
 
-lemma (in ast_problem) wf_lits_covered:
-  assumes "list_all1 wf_lit (un_and F)"
+lemma (in ast_classical_problem) wf_lits_covered:
+  assumes "(\<forall>x \<in> set (un_and F). wf_lit x)"
   shows "set (fmla_as_vars F) \<subseteq> set strips_vars"
   using assms wf_lit_covered unfolding fmla_as_vars_def by auto
 
-lemma (in ast_problem) wf_lits_goal_covered:
-  assumes "list_all1 wf_lit (un_and F)"
+lemma (in ast_classical_problem) wf_lits_goal_covered:
+  assumes "(\<forall>x \<in> set (un_and F). wf_lit x)"
   shows "fst ` set (fmla_as_goals F) \<subseteq> set strips_vars"
   using assms wf_lit_goal_covered apply simp
   using image_iff list.set_map subsetI by blast
 
-end text \<open>context ast_problem \<close>
+end text \<open>context ast_classical_problem \<close>
 
 lemma (in grounded_normalized_problem) wf_as_strips_op:
-  assumes "ac \<in> set (actions D)"
+  assumes "ac \<in> set (actions D)" "num_free_ac ac"
   shows "is_valid_operator_strips as_strips (as_strips_op ac)"
 proof -
   have C1: "\<forall>v\<in>set (precondition_of (as_strips_op ac)). v \<in> set strips_vars"
     using assms wf_pre_lits wf_lits_covered
     unfolding as_strips_op_sel by blast
 
-  obtain a d where eff: "ac_eff ac = Effect a d" by (cases "ac_eff ac") simp
+  obtain a d n where eff: "ac_eff ac = Effect a d n" by (cases "ac_eff ac") simp
 
   have "\<forall>v \<in> atm_as_vpos ` set a. v \<in> set strips_vars"
           "\<forall>v \<in> atm_as_vneg ` set a. v \<in> set strips_vars"
@@ -320,13 +377,13 @@ proof -
 
   have lits: "\<forall>x\<in>set ?adds. wf_lit_atom x"
     "\<forall>x\<in>set ?dels. wf_lit_atom x"
-    using wf_eff_lits[OF assms] apply (cases "ac_eff ac") apply simp_all
-    using wf_eff_lits[OF assms] apply (cases "ac_eff ac") apply simp_all
+    using wf_eff_lits[OF assms(1)] apply (cases "ac_eff ac") apply simp_all
+    using wf_eff_lits[OF assms(1)] apply (cases "ac_eff ac") apply simp_all
     done
   have v_inj: "x \<noteq> y \<Longrightarrow> wf_lit_atom x \<Longrightarrow> wf_lit_atom y \<Longrightarrow>
     atm_as_vpos x \<noteq> atm_as_vpos y \<and> atm_as_vneg x \<noteq> atm_as_vneg y" for x y
     apply (cases x rule: wf_lit.cases; cases y rule: wf_lit.cases; simp)
-    subgoal for u v apply (cases u; cases v) by simp done
+    subgoal for u v apply (cases u; cases v) by (simp add: lit_prepend_inj) done
 
   have adds_vs_dels: "atm_as_vpos ` set ?adds \<inter> atm_as_vpos ` set ?dels = {}" (is ?A)
           "atm_as_vneg ` set ?adds \<inter> atm_as_vneg ` set ?dels = {}" (is ?B)
@@ -346,7 +403,8 @@ proof -
       fix x y l assume "l = ?adds \<or> l = ?dels" "x \<in> set l" "y \<in> set l"
       hence "wf_lit_atom x" "wf_lit_atom y" by (auto simp add: lits)
       hence "atm_as_vneg x \<noteq> atm_as_vpos y"
-        by (cases x rule: is_predAtom.cases; cases y rule: is_predAtom.cases) simp_all
+        by (cases x rule: is_predAtom.cases; cases y rule: is_predAtom.cases)
+           (simp_all add: vneg_neq_vpos)
     }
     thus ?A ?B by force+
   qed
@@ -362,8 +420,12 @@ proof -
     unfolding as_strips_sel by blast    
 qed
 
-lemma (in grounded_problem) init_covered: "strips_init v \<noteq> None \<longleftrightarrow> v \<in> set strips_vars"
+locale grounded_normalized_numeric_free_problem =
+  grounded_normalized_problem + numeric_free_problem
+
+lemma (in grounded_normalized_numeric_free_problem) init_covered: "strips_init v \<noteq> None \<longleftrightarrow> v \<in> set strips_vars"
 proof -
+  have inf: "\<forall>f\<in>set (init P). num_free_fmla f" using num_free_prob unfolding num_free_prob_def by blast
   have "fold (\<lambda>v s. s(v \<mapsto> b)) vars s v \<noteq> None \<longleftrightarrow> v \<in> set vars \<or> s v \<noteq> None"
     for b vars s by (induction vars arbitrary: s) simp_all
   hence "empty_state v \<noteq> None \<longleftrightarrow> v \<in> set neg_vars \<or> v \<in> set pos_vars"
@@ -374,29 +436,37 @@ proof -
     (\<exists>x \<in> set vars. atm_as_vpos x = v \<or> atm_as_vneg x = v)" for vars s
     unfolding upd_init_def by (induction vars arbitrary: s) auto
   moreover have "\<exists>x \<in> set (init P). atm_as_vpos x = v \<or> atm_as_vneg x = v \<Longrightarrow> v \<in> set strips_vars"
-    using wf_init_lits wf_lit_atom_covered by auto
+    using wf_init_lits[OF inf] wf_lit_atom_covered by auto
   ultimately show ?thesis unfolding strips_init_def using empty by blast
 qed
 
-lemma (in grounded_normalized_problem) goal_covered:
+lemma (in grounded_normalized_numeric_free_problem) goal_covered:
   assumes "strips_goal v \<noteq> None"
   shows "v \<in> set strips_vars"
 proof -
+  have gnf: "num_free_fmla (goal P)" using num_free_prob unfolding num_free_prob_def by blast
   have "fold upd_goal xs s v \<noteq> None \<longleftrightarrow> s v \<noteq> None \<or> v \<in> fst ` set xs"
     for xs s apply (induction xs arbitrary: s) apply auto done
   hence "v \<in> fst ` set (fmla_as_goals (goal P))"
     using assms unfolding strips_goal_def by metis
-  thus ?thesis using wf_goal_lits wf_lits_goal_covered by blast
+  thus ?thesis using wf_goal_lits[OF gnf] wf_lits_goal_covered by blast
 qed
 
-theorem (in grounded_normalized_problem) wf_as_strips: "is_valid_problem_strips as_strips"
-  unfolding is_valid_problem_strips_def Let_def as_strips_sel
-  apply (intro conjI)
-  using wf_as_strips_op unfolding Ball_set[symmetric] apply simp
-  using init_covered apply (meson ListMem_iff)
-  using goal_covered by (meson ListMem_iff)
+theorem (in grounded_normalized_numeric_free_problem) wf_as_strips: "is_valid_problem_strips as_strips"
+proof -
+  have ndom: "\<forall>a\<in>set (actions D). num_free_ac a"
+    using num_free_prob unfolding num_free_prob_def num_free_dom_def by blast
+  have ops: "\<forall>ac\<in>set (actions D). is_valid_operator_strips as_strips (as_strips_op ac)"
+    using wf_as_strips_op ndom by blast
+  show ?thesis
+    unfolding is_valid_problem_strips_def Let_def as_strips_sel
+    apply (intro conjI)
+    using ops unfolding Ball_set[symmetric] apply simp
+    using init_covered apply (meson ListMem_iff)
+    using goal_covered by (meson ListMem_iff)
+qed
 
-sublocale grounded_normalized_problem \<subseteq> s: valid_strips as_strips
+sublocale grounded_normalized_numeric_free_problem \<subseteq> s: valid_strips as_strips
   using wf_as_strips by unfold_locales
 
 subsection \<open> STRIPS task semantics are preserved \<close>
@@ -404,18 +474,18 @@ subsection \<open> STRIPS task semantics are preserved \<close>
 lemma (in grounded_problem)
   "wf_pred n \<longleftrightarrow> PredDecl n [] \<in> set (predicates D)"
   "wf_pred n \<longleftrightarrow> n \<in> pred ` set (predicates D)"
-  "wf_pred n \<longleftrightarrow> vpos n \<in> pred_vpos ` set (predicates D)"
+  (* "wf_pred n \<longleftrightarrow> vpos n \<in> pred_vpos ` set (predicates D)" -- pred_vpos is iceboxed/undefined *)
     (* not pos_vars, tho, because n could be '''' and vpos n = v\<^sub>T *)
   oops
 
-context ast_problem begin
+context ast_classical_problem begin
 (* strips state equivalent *)
 
 term empty_state
 definition strips_model :: "world_model \<Rightarrow> name strips_state" where
   "strips_model M v \<equiv> undefined"
 
-thm wf_ast_domain.wf_empty_atom (* use this to work with wf_world_model M *)
+thm wf_ast_classical_domain.wf_empty_atom (* use this to work with wf_world_model M *)
 lemma strips_model_props:
   assumes "wf_world_model M"
     "wf_pred n"
@@ -424,8 +494,8 @@ lemma strips_model_props:
     "strips_model M v\<^sub>T = Some True"
     "strips_model M v\<^sub>F = Some False"
     "strips_model M v \<noteq> None \<longleftrightarrow> v \<in> set strips_vars"
-    "strips_model M (vpos n) = Some (Atom (predAtm n []) \<in> M)"
-    "strips_model M (vneg n) = Some (Atom (predAtm n []) \<notin> M)"
+    "strips_model M (vpos n) = Some (Atom (predAtm n []) \<in> fst M)"
+    "strips_model M (vneg n) = Some (Atom (predAtm n []) \<notin> fst M)"
   oops
 
 (* other direction equivalent *)
@@ -440,12 +510,12 @@ definition pddl_model :: "name strips_state \<Rightarrow> world_model" where
   "pddl_model s = undefined"
 lemma pddl_model_props:
   assumes "valid_strips_state s" "wf_pred n"
-  shows "Atom (predAtm n []) \<in> pddl_model s \<longleftrightarrow> s (vpos n) = Some True"
+  shows "Atom (predAtm n []) \<in> fst (pddl_model s) \<longleftrightarrow> s (vpos n) = Some True"
   oops
 
 
-fun (in ast_domain) strips_pa where
-  "strips_pa (PAction n args) = as_strips_op (the (resolve_action_schema n))"
+fun (in ast_classical_domain) strips_pa where
+  "strips_pa (SimplePlanAction n args) = as_strips_op (the (resolve_classical_action_schema n))"
 
 
 
@@ -464,5 +534,5 @@ corollary (in grounded_normalized_problem) valid_plan_iff:
   oops
 
 
-end text \<open> context ast_problem \<close>
-end
+end text \<open> context ast_classical_problem \<close>
+end  
