Base/STRIPS_Sema_Supplement.thy
@@ -1,12 +1,13 @@
 theory STRIPS_Sema_Supplement
   imports "Classical_Planning.Classical_Happening_Semantics"
+    "Verified_SAT_Based_AI_Planning.STRIPS_Representation"
 begin
 
 locale strips =
-  fixes \<Pi> :: "'a strips_problem"
+  fixes P_strips :: "'a strips_problem"
 
 locale valid_strips = strips +
-  assumes "is_valid_problem_strips \<Pi>"
+  assumes "is_valid_problem_strips P_strips"
 
 
 end
